theories/archival/Spec_indtype_spec_model.v
@@ -1,0 +1,735 @@
+
+(*** Modeling specs and morphisms as Coq terms ***)
+
+(* This approach defines an inductive type of specs and defines spec_model as a
+recursive function over specs that builds a nested dependent product *)
+
+
+Require Import List.
+Import ListNotations.
+Require Import String.
+
+(*
+Add LoadPath "." as Specware.
+Require Import Specware.Util.
+*)
+
+
+(*** Fields and Field Maps ***)
+
+(* We define the type of fields in one place, so we can change it later *)
+Definition Field : Set := string.
+Definition Field_dec : forall (f1 f2 : Field), {f1=f2} + {f1<>f2} := string_dec.
+
+Lemma Field_dec_eq f : { e : f = f | Field_dec f f = left e }.
+  destruct (Field_dec f f).
+  exists e; reflexivity.
+  elimtype False; apply n; reflexivity.
+Qed.
+
+Lemma Field_dec_neq f f' : f <> f' -> { neq : f <> f' | Field_dec f f' = right neq }.
+  destruct (Field_dec f f'); intros.
+  elimtype False; apply (H e).
+  exists n; reflexivity.
+Qed.
+
+
+(* A field map is an association list on fields *)
+Definition FMap := list (Field * Field).
+
+(*
+Definition FMap := { l : list (Field * Field) | NoDup (map fst l) }.
+
+Lemma NoDup_tail A (x:A) l : NoDup (x::l) -> NoDup l.
+  intro nd. apply (NoDup_remove_1 [] l x). assumption.
+Qed.
+*)
+
+(* Apply a field map to a field *)
+Fixpoint apply_fmap (m : FMap) (f : Field) : Field :=
+  match m with
+    | [] => f
+    | (f_in, f_out) :: m' =>
+      if Field_dec f f_in then f_out else apply_fmap m' f
+  end.
+
+(* The identity field map *)
+Definition fmap_id : FMap := [].
+
+(* fmap_id is the identity *)
+Lemma fmap_id_ok f : apply_fmap fmap_id f = f.
+  reflexivity.
+Qed.
+
+(* Compose two field maps *)
+Fixpoint fmap_compose (m2 m1 : FMap) : FMap :=
+  match m1 with
+    | [] => m2
+    | (f_in, f_out) :: m1' =>
+      (f_in, apply_fmap m2 f_out) :: fmap_compose m2 m1'
+  end.
+
+(* Field map composition commutes with application *)
+Lemma fmap_compose_ok m2 m1 f :
+  apply_fmap (fmap_compose m2 m1) f = apply_fmap m2 (apply_fmap m1 f).
+  induction m1.
+  reflexivity.
+  destruct a.
+  unfold apply_fmap; unfold fmap_compose; fold fmap_compose; fold apply_fmap.
+  destruct (Field_dec f f0).
+  reflexivity.
+  assumption.
+Qed.
+
+(* The domain of a field map *)
+Definition fmap_dom (m : FMap) : list Field := map fst m.
+
+(* Inversion lemma for field maps *)
+(*
+Lemma reverse_fmap m f1 f2 :
+  apply_fmap m f1 = f2 -> f1 = f2 \/ In f1 (fmap_dom m).
+  admit. (* FIXME HERE *)
+Qed.
+*)
+
+
+(*** Field lists, with no duplicates ***)
+
+Definition flist := { l : list Field | NoDup l }.
+
+Definition fnil : flist := exist _ [] (NoDup_nil Field).
+
+Definition fcons f l (pf : ~ In f (proj1_sig l)) : flist :=
+  exist _ (f :: proj1_sig l) (NoDup_cons f pf (proj2_sig l)).
+
+Definition in_fl f (l : flist) : Prop := In f (proj1_sig l).
+
+Definition in_fl_dec f l : {in_fl f l} + {~ in_fl f l} :=
+  In_dec Field_dec f (proj1_sig l).
+
+Lemma in_fl_eq f l pf : in_fl f (fcons f l pf).
+  left; reflexivity.
+Qed.
+
+Lemma in_fl_fcons_inv f f' l pf : in_fl f (fcons f' l pf) -> f' <> f -> in_fl f l.
+  unfold in_fl; intros; destruct H.
+    elimtype False; apply (H0 H).
+    assumption.
+Qed.
+
+Definition in_fl_inv f f' l pf (i: in_fl f (fcons f' l pf)) : {f'=f} + {in_fl f l} :=
+  match Field_dec f' f with
+    | left e => left e
+    | right neq => right (in_fl_fcons_inv _ _ _ _ i neq)
+  end.
+
+
+(*** The inductive type of specs ***)
+
+Inductive Spec : flist -> Type :=
+(* The base case contains the names and types of the axioms *)
+| Spec_Axioms (axioms : list (Field * Prop)) : Spec fnil
+(* Declared op: the rest of the spec can refer to the op *)
+| Spec_DeclOp f flds not_in (T : Type) (rest : T -> Spec flds)
+  : Spec (fcons f flds not_in)
+(* Defined op: gives an element of the type *)
+| Spec_DefOp f flds not_in (T : Type) (t : T) (rest : Spec flds)
+  : Spec (fcons f flds not_in)
+.
+
+(* Helper for building the type of the "rest" of a spec_cons *)
+Definition spec_rest flds T (t_opt:option T) : Type :=
+  match t_opt with
+    | Some (_) => Spec flds
+    | None => T -> Spec flds
+  end.
+
+(* Helper for consing declared or defined ops *)
+Definition spec_cons f flds not_in T t_opt :
+  (spec_rest flds T t_opt) -> Spec (fcons f flds not_in) :=
+  match t_opt return spec_rest flds T t_opt -> Spec (fcons f flds not_in) with
+    | Some t =>
+      Spec_DefOp f flds not_in T t
+    | None =>
+      Spec_DeclOp f flds not_in T
+  end.
+
+(* Helper for building the type of the "rest" of a spec_cons *)
+(*
+Definition spec_rest_arg T (t_opt:option T) : Type :=
+  match t_opt with
+    | Some (_) => Spec flds
+    | None => T -> Spec flds
+  end.
+*)
+
+(* Helper for applying the "rest" of a spec_cons to an optional argument *)
+(*
+Definition spec_rest_apply flds T t_opt :
+  spec_rest flds T t_opt -> Spec flds :=
+  match t_opt return spec_rest flds T t_opt -> Spec flds with
+    | Some t => fun rest => rest t
+    | None => fun rest => rest
+  end.
+*)
+
+(*** The Models of a Spec ***)
+
+(* Helper for elements of a model at an arbitrary type *)
+Definition Any : Type := { T : Type & T }.
+Definition mkAny (T:Type) (t:T) : Any := existT (fun T => T) T t.
+
+(* Helper for conjoining all the axioms in an axiom list *)
+Fixpoint conjoin_axioms (axioms : list (Field * Prop)) : Prop :=
+  fold_left (fun P1 f_P2 => and P1 (snd f_P2)) axioms True.
+
+(* Build the type of the models of spec as a nested dependent pair *)
+Fixpoint spec_model flds (spec:Spec flds) : Type :=
+  match spec in Spec flds with
+    | Spec_Axioms axioms =>
+      conjoin_axioms axioms
+    | Spec_DeclOp _ flds' _ T rest =>
+      { t : T & spec_model flds' (rest t)}
+    | Spec_DefOp _ flds' _ _ _ rest => spec_model flds' rest
+  end.
+
+(* Whether field f has type T in a model *)
+Fixpoint has_type_in_model f T flds spec : spec_model flds spec -> Prop :=
+  match spec in Spec flds return spec_model flds spec -> Prop with
+    | Spec_Axioms _ => fun model => False
+    | Spec_DeclOp f' flds' not_in T' rest =>
+      fun model =>
+        (f = f' -> T' = T) /\
+        (f <> f' ->
+         has_type_in_model f T flds' (rest (projT1 model)) (projT2 model))
+    | Spec_DefOp f' flds' not_in T' t' rest =>
+      fun model =>
+        (f = f' -> T' = T) /\
+        (f <> f' -> has_type_in_model f T flds' rest model)
+  end.
+
+Lemma has_type_in_model_in_flds f T flds spec model :
+  has_type_in_model f T flds spec model -> in_fl f flds.
+  revert model; induction spec; intros.
+  elimtype False; apply H.
+  destruct (Field_dec f f0).
+  rewrite e; apply in_fl_eq.
+  right. apply (H (projT1 model) (projT2 model)).
+  destruct H0. apply H1. assumption.
+  destruct (Field_dec f f0).
+  rewrite e; apply in_fl_eq.
+  right; apply (IHspec model). destruct H. apply H0. assumption.
+Qed.
+
+Lemma has_type_in_model_eq f T flds not_in t_opt rest model :
+  has_type_in_model f T _ (spec_cons f flds not_in T t_opt rest) model.
+  destruct t_opt; (split; intros; [ | elimtype False; apply H ]; reflexivity).
+Qed.
+
+Lemma has_type_in_model_cons f T f' flds' not_in T' t_opt' rest model
+: f <> f' -> has_type_in_model f T flds' (rest t') model ->
+  has_type_in_model f T _ (Spec_DeclOp f' flds' not_in T' rest) (existT _ t' model).
+  split; [ intro H1; elimtype False; apply (H H1) | ].
+  intros; assumption.
+Qed.
+
+Lemma has_type_in_model_cons_decl f T f' flds' not_in T' t' rest model
+: f <> f' -> has_type_in_model f T flds' (rest t') model ->
+  has_type_in_model f T _ (Spec_DeclOp f' flds' not_in T' rest) (existT _ t' model).
+  split; [ intro H1; elimtype False; apply (H H1) | ].
+  intros; assumption.
+Qed.
+
+Lemma has_type_in_model_cons_def f T f' flds' not_in T' t' rest model
+: f <> f' -> has_type_in_model f T flds' rest model ->
+  has_type_in_model f T _ (Spec_DefOp f' flds' not_in T' t' rest) model.
+  split; [ intro H1; elimtype False; apply (H H1) | ].
+  intros; assumption.
+Qed.
+
+
+(* Project a field out of a model of a spec *)
+Fixpoint model_proj f T flds spec
+: forall model, has_type_in_model f T flds spec model -> T :=
+  match spec in Spec flds
+        return forall model, has_type_in_model f T flds spec model -> T with
+    | Spec_Axioms _ => fun model htim => (match htim with end)
+    | Spec_DeclOp f' flds' not_in T' rest =>
+      fun model htim =>
+        match Field_dec f f' with
+          | left e => eq_rect T' id (projT1 model) T
+                              ((match htim with conj f _ => f end) e)
+          | right neq =>
+            model_proj f T flds' (rest (projT1 model)) (projT2 model)
+                       ((match htim with conj _ f => f end) neq)
+        end
+    | Spec_DefOp f' flds' not_in T' t rest =>
+      fun model htim =>
+        match Field_dec f f' with
+          | left e => eq_rect T' id t T
+                              ((match htim with conj f _ => f end) e)
+          | right neq => model_proj f T flds' rest model
+                                    ((match htim with conj _ f => f end) neq)
+        end
+  end.
+
+(*
+Fixpoint model_proj f flds spec : in_fl f flds -> spec_model flds spec -> Any :=
+  match spec in Spec flds
+        return in_fl f flds -> spec_model flds spec -> Any with
+    | Spec_Axioms _ => fun i _ => (match i with end)
+    | Spec_DeclOp f' flds' not_in T rest =>
+      fun i model =>
+        match in_fl_inv f f' flds' not_in i with
+          | left _ => mkAny T (projT1 model)
+          | right i' => model_proj f flds' (rest (projT1 model)) i' (projT2 model)
+        end
+    | Spec_DefOp f' flds' not_in T t rest =>
+      fun i model =>
+        match in_fl_inv f f' flds' not_in i with
+          | left _ => mkAny T t
+          | right i' => model_proj f flds' rest i' model
+        end
+  end.
+*)
+
+
+(*** Model Substitution ***)
+
+(* This is true iff a model of source can be built from a given model of target
+by using field map m to map each field of source to one of target. *)
+Fixpoint CanSubstModel (m : FMap) flds_s (source : Spec flds_s) flds_t
+         (target : Spec flds_t) (model : spec_model _ target) : Prop :=
+  match source in Spec flds_s with
+    | Spec_Axioms axioms => conjoin_axioms axioms
+    | Spec_DeclOp f flds_s' not_in T rest =>
+      exists (htim : has_type_in_model (apply_fmap m f) T flds_t target model),
+        CanSubstModel m flds_s' (rest (model_proj _ _ _ _ model htim)) flds_t target model
+    | Spec_DefOp f flds_s' not_in T t rest =>
+      exists (htim : has_type_in_model (apply_fmap m f) T flds_t target model),
+        model_proj _ _ _ _ model htim = t /\
+        CanSubstModel m flds_s' rest flds_t target model
+  end.
+
+(*
+Inductive CanSubstModel (m : FMap) flds_t target (model : spec_model flds_t target) : 
+  forall flds_s, Spec flds_s -> Prop :=
+| CanSubst_Axioms axioms (pf : conjoin_axioms axioms)
+  : CanSubstModel m flds_t target model fnil (Spec_Axioms axioms)
+| CanSubst_DeclOp f flds_s not_in T rest t i
+                  (e : model_proj (apply_fmap m f) _ _ i model = mkAny T t)
+                  (rec : CanSubstModel m flds_t target model flds_s (rest t))
+  : CanSubstModel m flds_t target model _
+                  (Spec_DeclOp f flds_s not_in T rest)
+| CanSubst_DefOp f flds_s not_in T rest t i
+                  (e : model_proj (apply_fmap m f) _ _ i model = mkAny T t)
+                  (rec : CanSubstModel m flds_t target model flds_s rest)
+  : CanSubstModel m flds_t target model _
+                  (Spec_DefOp f flds_s not_in T t rest)
+.
+*)
+
+Lemma CanSubstModel_cons_decl m f flds_t not_in T t target model flds_s source
+: CanSubstModel m flds_s source flds_t (target t) model ->
+  CanSubstModel m flds_s source _ (Spec_DeclOp f flds_t not_in T target) (existT _ t model).
+  induction source; unfold CanSubstModel; fold CanSubstModel; intro csm.
+  assumption.
+  destruct csm as [htim csm].
+  assert (apply_fmap m f0 <> f) as neq.
+    intro; apply not_in; rewrite <- H0;
+      apply (has_type_in_model_in_flds _ _ _ _ _ htim).
+  assert (apply_fmap m f0 = f -> T = T0); [ intros; contradiction | ].
+  exists (conj H0 (fun _ => htim)).
+  unfold model_proj; fold model_proj.
+  destruct (Field_dec_neq _ _ neq); rewrite e. apply H. assumption.
+  destruct csm as [htim conj]; destruct conj as [proj_eq csm].
+  assert (apply_fmap m f0 <> f) as neq.
+    intro; apply not_in; rewrite <- H;
+      apply (has_type_in_model_in_flds _ _ _ _ _ htim).
+  assert (apply_fmap m f0 = f -> T = T0); [ intros; contradiction | ].
+  exists (conj H (fun _ => htim)).
+  unfold model_proj; fold model_proj.
+  destruct (Field_dec_neq _ _ neq); rewrite e. split.
+  assumption.
+  apply IHsource. assumption.
+Qed.
+
+Lemma CanSubstModel_cons_def m f flds_t not_in T t target model flds_s source
+: CanSubstModel m flds_s source flds_t target model ->
+  CanSubstModel m flds_s source _ (Spec_DefOp f flds_t not_in T t target) model.
+  induction source; unfold CanSubstModel; fold CanSubstModel; intro csm.
+  assumption.
+  destruct csm as [htim csm].
+  assert (apply_fmap m f0 <> f) as neq.
+    intro; apply not_in; rewrite <- H0;
+      apply (has_type_in_model_in_flds _ _ _ _ _ htim).
+  assert (apply_fmap m f0 = f -> T = T0); [ intros; contradiction | ].
+  exists (conj H0 (fun _ => htim)).
+  unfold model_proj; fold model_proj.
+  destruct (Field_dec_neq _ _ neq); rewrite e. apply H. assumption.
+  destruct csm as [htim conj]; destruct conj as [proj_eq csm].
+  assert (apply_fmap m f0 <> f) as neq.
+    intro; apply not_in; rewrite <- H;
+      apply (has_type_in_model_in_flds _ _ _ _ _ htim).
+  assert (apply_fmap m f0 = f -> T = T0); [ intros; contradiction | ].
+  exists (conj H (fun _ => htim)).
+  unfold model_proj; fold model_proj.
+  destruct (Field_dec_neq _ _ neq); rewrite e. split.
+  assumption.
+  apply IHsource. assumption.
+Qed.
+
+
+(* CanSubstModel is reflexive *)
+Lemma CanSubstModel_refl flds spec model : CanSubstModel fmap_id flds spec flds spec model.
+  revert model; induction spec; intros.
+  assumption.
+  unfold CanSubstModel; fold CanSubstModel; rewrite fmap_id_ok.
+  unfold model_proj; fold model_proj.
+  destruct (Field_dec_eq f). rewrite e.
+  destruct model as [t model].
+  assert (f <> f -> has_type_in_model f T flds (rest t) model).
+  intro neq; elimtype False; apply neq; reflexivity.
+  exists (conj (fun _ => eq_refl) H0).
+  apply CanSubstModel_cons_decl. apply H.
+  unfold CanSubstModel; fold CanSubstModel; rewrite fmap_id_ok.
+  unfold model_proj; fold model_proj.
+  destruct (Field_dec_eq f). rewrite e.
+  assert (f <> f -> has_type_in_model f T flds spec model).
+  intro neq; elimtype False; apply neq; reflexivity.
+  exists (conj (fun _ => eq_refl) H).
+  split; [ reflexivity | ].
+  apply CanSubstModel_cons_def. apply IHspec.
+Qed.
+
+
+(* Perform model substitution. This intuitively applies the map m backwards,
+building a model of source from a model of target by applying m to each field in
+source to get the field name for the value to use in the model of target. *)
+Fixpoint subst_model m flds_s source flds_t target model :
+  CanSubstModel m flds_s source flds_t target model -> spec_model flds_s source :=
+  match source in Spec flds_s
+        return CanSubstModel m flds_s source flds_t target model ->
+               spec_model flds_s source with
+    | Spec_Axioms axioms =>
+      fun pf => pf
+    | Spec_DeclOp f flds_s' not_in T rest =>
+      fun can_subst =>
+        existT (fun t => spec_model _ (rest t))
+               (model_proj (apply_fmap m f) T flds_t target model
+                           (match can_subst with ex_intro ))
+               (subst_model m _ target model (proj2_sig can_subst))
+    | Spec_DefOp f flds_s' not_in T t rest =>
+      fun can_subst =>
+        (subst_model m _ target model
+                     (proj2 (proj2_sig can_subst)))
+  end.
+
+
+
+
+(*** FIXME: Old Stuff Below ***)
+
+
+(* Whether field f has type T in a given model of spec *)
+Fixpoint field_has_type f T spec : spec_model spec -> Prop :=
+  match spec return spec_model spec -> Prop with
+    | Spec_Axioms _ => fun model => False
+    | Spec_DeclOp f' T' rest =>
+      fun model =>
+        if Field_dec f f' then T' = T else
+          field_has_type f T (rest (projT1 model)) (projT2 model)
+    | Spec_DefOp f' T' t rest =>
+      fun model =>
+        if Field_dec f f' then T' = T else
+          field_has_type f T rest model
+  end.
+
+(* Invert field_has_type for Spec_DeclOp *)
+Definition field_has_type_inv_decl f T f' T' rest :
+  forall model,
+    field_has_type f T (Spec_DeclOp f' T' rest) model ->
+    {T' = T} + {field_has_type f T (rest (projT1 model)) (projT2 model)}.
+  unfold field_has_type; fold field_has_type; unfold spec_model; fold spec_model.
+  destruct (Field_dec f f'); intros.
+  left; assumption.
+  right; assumption.
+Defined.
+
+(* Invert field_has_type for Spec_DefOp *)
+Definition field_has_type_inv_def f T f' T' t' rest :
+  forall model,
+    field_has_type f T (Spec_DefOp f' T' t' rest) model ->
+    {T' = T} + {field_has_type f T rest model}.
+  unfold field_has_type; fold field_has_type; unfold spec_model; fold spec_model.
+  destruct (Field_dec f f'); intros.
+  left; assumption.
+  right; assumption.
+Defined.
+
+
+(* Project a named field out of a model of a spec *)
+(*
+Definition model_proj f T spec :
+  forall (model:spec_model spec), field_has_type f T spec model -> T.
+  induction spec; unfold field_has_type; fold field_has_type;
+    unfold spec_model; fold spec_model.
+  intros; elimtype False; assumption.
+  destruct (Field_dec f f0).
+    intros; rewrite <- H; apply (projT1 model).
+    intros; apply (X (projT1 model) (projT2 model)); assumption.
+  destruct (Field_dec f f0).
+    intros; rewrite <- H; apply t.
+    intros; apply (IHspec model); assumption.
+Defined.
+*)
+
+Fixpoint model_proj f T spec :
+  forall (model:spec_model spec), field_has_type f T spec model -> T :=
+  match spec return forall (model:spec_model spec),
+                      field_has_type f T spec model -> T with
+    | Spec_Axioms _ =>
+      fun model has_type => (match has_type with end)
+    | Spec_DeclOp f' T' rest =>
+      fun model has_type =>
+        (match field_has_type_inv_decl f T f' T' rest model has_type with
+           | left e => eq_rect T' id (projT1 model) T e
+           | right has_type' =>
+             model_proj f T (rest (projT1 model)) (projT2 model) has_type'
+         end)
+    | Spec_DefOp f' T' t' rest =>
+      fun model has_type =>
+        (match field_has_type_inv_def f T f' T' t' rest model has_type with
+           | left e => eq_rect T' id t' T e
+           | right has_type' =>
+             model_proj f T rest model has_type'
+         end)
+  end.
+
+
+(*** Model Substitution ***)
+
+(* This is true iff a model of source can be built from a given model of target
+by using field map m to map each field of source to one of target. *)
+Fixpoint CanSubstModel (m : FMap) (source target : Spec)
+         (model : spec_model target) : Prop :=
+  match source with
+    | Spec_Axioms axioms => conjoin_axioms axioms
+    | Spec_DeclOp f T rest =>
+      { has_type:field_has_type (apply_fmap m f) T target model |
+        CanSubstModel m (rest (model_proj (apply_fmap m f) T target model has_type))
+                      target model }
+    | Spec_DefOp f T t rest =>
+      { has_type:field_has_type (apply_fmap m f) T target model |
+        (model_proj (apply_fmap m f) T target model has_type) = t /\
+        CanSubstModel m rest target model }
+  end.
+
+(* Perform model substitution. This intuitively applies the map m backwards,
+building a model of source from a model of target by applying m to each field in
+source to get the field name for the value to use in the model of target. *)
+Fixpoint subst_model m source target model :
+  CanSubstModel m source target model -> spec_model source :=
+  match source return CanSubstModel m source target model -> spec_model source with
+    | Spec_Axioms axioms =>
+      fun pf => pf
+    | Spec_DeclOp f T rest =>
+      fun can_subst =>
+        existT (fun t => spec_model (rest t))
+               (model_proj (apply_fmap m f) T target model (proj1_sig can_subst))
+               (subst_model m _ target model (proj2_sig can_subst))
+    | Spec_DefOp f T t rest =>
+      fun can_subst =>
+        (subst_model m _ target model
+                     (proj2 (proj2_sig can_subst)))
+  end.
+
+(* CanSubstModel is reflexive *)
+Lemma CanSubstModel_refl spec model : CanSubstModel fmap_id spec spec model.
+  revert model; induction spec; unfold CanSubstModel; unfold spec_model;
+    fold spec_model; fold CanSubstModel.
+  intros; assumption.
+  rewrite fmap_id_ok; intro model; destruct model as [t model].
+  assert (field_has_type f T (Spec_DeclOp f T rest) (existT _ t model)) as has_type.
+  unfold field_has_type; fold field_has_type;
+    destruct (Field_dec_eq f) as [eq_f_f eq_field_dec]; rewrite eq_field_dec; reflexivity.
+  exists has_type. unfold CanSubstModel; fold CanSubstModel.
+
+  assert {e:Field_dec f f}
+
+  unfold model_proj; unfold field_has_type_inv_decl; unfold projT1; unfold projT2;
+fold (model_proj f T);
+  destruct (Field_dec f f).
+  Focus 2. fold (model_proj f T (Spec_Decl)).
+
+exists (eq_refl T).
+
+
+(*** Morphisms ***)
+
+(* Field map m is a morphism from source to target iff it can be used to
+substitute into any model of target to get a model of source *)
+Definition IsMorphism (m : FMap) (source target : Spec) : Prop :=
+  forall (model:spec_model target), CanSubstModel m source target model.
+
+
+
+
+(*** FIXME: old stuff below ***)
+
+(*** The models of a spec ***)
+
+Definition Any : Type := { T : Type & T }.
+Definition mkAny (T:Type) (t:T) : Any := existT (fun T => T) T t.
+Definition dummyAny : Any := mkAny _ tt.
+
+Definition Model := list (Field * Any).
+
+Fixpoint model_proj f model : option Any :=
+  match model with
+    | [] => None
+    | (f', any) :: model' =>
+      if Field_dec f f' then Some any else
+        model_proj f model'
+  end.
+
+(* NOTE: this is in Type because we need to compute the model elements *)
+Fixpoint IsModel (model:Model) (s:Spec) : Prop :=
+  match s with
+    | Spec_Axioms axioms => conjoin_axioms axioms
+    | Spec_DeclOp f T rest =>
+      exists t, model_proj f model = Some (mkAny T t) /\ IsModel model (rest t)
+    | Spec_DefOp f T t rest =>
+      model_proj f model = Some (mkAny T t) /\ IsModel model rest
+  end.
+
+
+(*** Morphisms ***)
+
+Fixpoint unmap_model (m : FMap) (model:Model) : Model := FIXME HERE
+
+Fixpoint IsMappedModel (m : FMap) (model:Model) (s:Spec) : Prop :=
+  match s with
+    | Spec_Axioms axioms => conjoin_axioms axioms
+    | Spec_DeclOp f T rest =>
+      exists t,
+        model_proj (apply_fmap m f) model = Some (mkAny T t)
+        /\ IsMappedModel m model (rest t)
+    | Spec_DefOp f T t rest =>
+      model_proj (apply_fmap m f) model = Some (mkAny T t)
+      /\ IsMappedModel m model rest
+  end.
+
+Definition IsMorphism m (source target : Spec) : Prop :=
+  forall model, IsModel model target -> IsMappedModel m model source.
+
+
+Lemma IsMappedModel_id model s : IsModel model s <-> IsMappedModel fmap_id model s.
+  split; induction s;
+  unfold IsModel; fold IsModel; unfold IsMappedModel; fold IsMappedModel; intro.
+  assumption.
+  destruct H0; destruct H0; exists x; split; [ | apply H]; assumption.
+  destruct H; split; [ | apply IHs ]; assumption.
+  assumption.
+  destruct H0; destruct H0; exists x; split; [ | apply H]; assumption.
+  destruct H; split; [ | apply IHs ]; assumption.
+Qed.
+
+Theorem morphism_refl spec : IsMorphism fmap_id spec spec.
+  intros model ism; apply IsMappedModel_id; assumption.
+Qed.
+
+(* Need a model (or a mapped model) to extract the fields from a spec *)
+(* Argh, needs UIP! *)
+(*
+Definition spec_fields m model spec : IsMappedModel m model spec -> list Field.
+  induction spec; unfold IsMappedModel; fold IsMappedModel; intro ism.
+  exact [].
+  destruct (model_proj (m f) model).
+  destruct a. assert (x = T).
+  destruct ism; destruct H; injection H; intros; assumption.
+  revert p ism; rewrite H; intros.
+  assert (IsMappedModel m model (rest p)).
+  destruct ism; 
+*)
+(*
+Fixpoint spec_fields m model spec : IsMappedModel m model spec -> list Field :=
+  match spec with
+    | Spec_Axioms _ => fun _ => []
+    | Spec_DeclOp f T rest =>
+*)
+
+
+Definition unmap_model (m : Field -> Field) (model:Model) (s:Spec) :
+  IsMappedModel m model s -> {model' | IsModel model' s }.
+  induction s; unfold IsMappedModel; fold IsMappedModel;
+  unfold IsModel; fold IsModel; intro ism.
+  exists []; assumption.
+  case_eq (model_proj (m f) model); intros.
+  destruct a. assert (x = T).
+  destruct ism; destruct H0; rewrite H in H0;
+    injection H0; intros; assumption.
+  revert p H; rewrite H0; intros.
+  destruct (X p).
+  
+
+  exists (m f, a).
+
+
+Fixpoint unmap_model (m : Field -> Field) (model:Model) (s:Spec) :
+  IsMappedModel m model s -> Model :=
+  match s with
+    | Spec_Axioms axioms => fun _ => x[]
+    | Spec_DeclOp f T rest =>
+      fun ism =>
+
+
+(*** FIXME: Old stuff below... ***)
+
+Fixpoint spec_model (spec:Spec) : Type :=
+  match spec with
+    | Spec_Axioms axioms =>
+      conjoin_axioms axioms
+    | Spec_DeclOp _ T rest =>
+      { t : T & spec_model (rest t)}
+    | Spec_DefOp _ _ _ rest => spec_model rest
+  end.
+
+
+(*** Project an op from a model of a spec ***)
+
+Fixpoint model_proj f spec : spec_model spec -> { T : Type & T } :=
+  match spec  with
+    | Spec_Axioms _ => fun _ => existT (fun T => T) unit tt
+    | Spec_DeclOp f' T rest =>
+      fun model =>
+        if Field_dec f f' then (existT (fun T => T) T (projT1 model))
+      else model_proj f (rest (projT1 model)) (projT2 model)
+    | Spec_DefOp f' T t rest =>
+      fun model =>
+        if Field_dec f f' then existT _ T t
+        else model_proj f rest model
+  end.
+
+
+(*** Whether a field function defines a morphism ***)
+
+(* Note: the co-domain comes first in IsMorphism, because it does not vary *)
+(*
+Inductive IsMorphism (m : Field -> Field) (s_codom : Spec) : Spec -> Prop :=
+| IsMorphism_Axioms 
+*)
+
+Fixpoint IsMorphModel (m : Field -> Field)
+         (source target : Spec) (t_model : Model) : Prop :=
+  match source with
+    | Spec_Axioms axioms =>
+      conjoin_axioms axioms
+    | Spec_DeclOp f T rest =>
+      
+
+Fixpoint IsMorphism (m : Field -> Field) (source target : Spec) : Prop :=
+  match source with
+    | Spec_Axioms axioms =>
+      conjoin_axioms axioms
+    | Spec_DeclOp f T rest =>
